added lookupLT, lookupLE, and varieties of insertion

examples/containers/theories/MapProofs.v
@@ -1273,6 +1273,460 @@ Proof.
   destruct H3. rewrite H3 in H. inversion H.
 Qed.
 
+(** ** Verification of [findWithDefault] *)
+Lemma findWithDefault_spec:
+  forall {m lb ub i v}, Bounded m lb ub -> 
+  Some (findWithDefault v i m) = sem m i ||| Some v.
+Proof.
+  intros. induction H.
+  - simpl. reflexivity.
+  - simpl. destruct (compare i x) eqn : ?.
+    + assert (sem s1 i = None). { eapply sem_outside_above. eassumption. solve_Bounds. }
+      rewrite H5. assert (i == x = true) by (order e). rewrite H6. reflexivity.
+    + assert (i == x = false) by (order e). assert (sem s2 i = None). { eapply sem_outside_below.
+      eassumption. solve_Bounds. } rewrite H5. rewrite H6. simpl. rewrite oro_None_r.
+      rewrite oro_None_r. apply IHBounded1.
+    + assert (i == x = false) by (order e). assert (sem s1 i = None). { eapply sem_outside_above.
+      eassumption. solve_Bounds. } rewrite H5. rewrite H6. simpl. apply IHBounded2.
+Qed.
+(** ** Verification of [lookupLT] *)
+Fixpoint goJustLT k  (k1: e) v1 (m : Map e a) : option (e * a) :=
+  match m with
+  | Tip => Some (k1, v1)
+  | Bin sz k2 v2 l r => if (_GHC.Base.<=_ k k2) then goJustLT k k1 v1 l else
+    goJustLT k k2 v2 r 
+  end.
+Fixpoint lookupLT' k (m : Map e a) :=
+  match m with
+  | Tip => None
+  | Bin sz k1 v1 l r => if (_GHC.Base.<=_ k k1) then lookupLT' k l else goJustLT k k1 v1 r
+  end.
+
+Lemma lookupLT_equiv:
+  forall m k,
+  lookupLT' k m = lookupLT k m.
+Proof.
+  intros. unfold lookupLT'. unfold lookupLT. unfold goJustLT. reflexivity.
+Qed.
+
+Lemma goJustLT_pres_smaller: forall k k1 v1 m k2 v2 lb ub,
+  Bounded m lb ub ->
+  _GHC.Base.<_ k1 k = true ->
+  goJustLT k k1 v1 m = Some (k2, v2) ->
+  _GHC.Base.<_ k2 k = true.
+Proof.
+  intros. generalize dependent k1. revert v1 v2 k2 k. induction H; intros.
+  - simpl in H1. inversion H1; subst. assumption.
+  - simpl in H6. destruct (_GHC.Base.<=_ k x) eqn : ?.
+   + eapply IHBounded1. eassumption. eassumption.
+   + assert (_GHC.Base.<_ x k = true) by (order e). eapply IHBounded2. apply H7.
+      apply H6.
+Qed.
+
+Lemma goJustLT_bounded: forall k k1 v1 m k2 v2 lb ub l u,
+  Bounded m lb ub ->
+  _GHC.Base.<_ k1 k = true ->
+  goJustLT k k1 v1 m = Some (k2, v2) ->
+  (lb = Some l /\ _GHC.Base.<=_ l k1 = true -> _GHC.Base.<=_ l k2 = true ) 
+  /\ (ub = Some u /\ _GHC.Base.<=_ k1 u = true -> _GHC.Base.<=_ k2 u = true).
+Proof.
+  intros. generalize dependent k1. revert k v1 k2 v2 u l. induction H; intros.
+  - simpl in H1. inversion H1; subst. split; intros; subst; solve_Bounds.
+  - simpl in H6. destruct (_GHC.Base.<=_ k x) eqn : ?. 
+    + split; intros; subst.  specialize (IHBounded1 _ _ _ _ u l _ H5 H6). destruct IHBounded1.
+       apply H3. apply H7. specialize (IHBounded1 _ _ _ _ x l  _ H5 H6). destruct IHBounded1.
+        destruct H7; subst. assert (Some x = Some x /\ _GHC.Base.<=_ k1 x = true).
+        split. reflexivity. order e. apply H8 in H7.  assert (compare x u = Lt) by (solve_Bounds). 
+        order e.
+    + assert (_GHC.Base.<_ x k = true) by (order e).  split; intros; subst. 
+      specialize (IHBounded2  _ _ _ _ u x _ H7 H6). destruct IHBounded2. 
+      destruct H8; subst. assert (_GHC.Base.<=_ x k2 = true). apply H3. split. reflexivity.
+      order e. assert (_GHC.Base.<_ l x = true) by (solve_Bounds). order e.
+      specialize (IHBounded2 _ _ _ _ u l _ H7 H6). destruct IHBounded2. apply H9.
+      split. apply H8. destruct H8. subst. solve_Bounds.
+Qed. 
+
+Lemma goJustLT_nothing_between: forall k k1 v1 m lb ub k2 v2,
+  Bounded m lb ub ->
+  _GHC.Base.<_ k1 k = true ->
+  goJustLT k k1 v1 m = Some (k2, v2) ->
+  (forall i, compare k2 i = Lt /\ compare i k = Lt ->
+  sem m i = None).
+Proof.
+  intros. generalize dependent i. generalize dependent k2. generalize dependent k1.
+  revert k v1 v2.
+  induction H; intros.
+  - reflexivity.
+  - simpl. simpl in H6. destruct ( _GHC.Base.<=_ k x) eqn : ?.
+    + assert (i == x = false) by (order e). rewrite H8. assert (sem s2 i = None). {
+      eapply sem_outside_below. eassumption. solve_Bounds. } rewrite H9.
+      simpl. repeat(rewrite oro_None_r). eapply IHBounded1. apply H5. apply H6.
+      assumption.
+    + assert (_GHC.Base.<_ x k = true) by (order e).
+      pose proof goJustLT_bounded. specialize (H9 _ _ _ _ _ _ _ _ x k H0 H8 H6).
+      destruct H9. assert (_GHC.Base.<=_ x k2 = true). apply H9. split. reflexivity.
+      order e. assert (_GHC.Base.<_ x i = true). order e. assert (sem s1 i = None).
+      eapply sem_outside_above. eassumption. solve_Bounds. rewrite H13.
+      assert (i == x = false) by (order e). rewrite H14. simpl. eapply IHBounded2.
+      apply H8. apply H6. apply H7.
+Qed.
+
+Lemma goJustLT_finds_upper_bound: forall k k1 v1 m lb ub k2 v2,
+  Bounded m lb ub ->
+  _GHC.Base.<_ k1 k = true ->
+  goJustLT k k1 v1 m = Some (k2, v2) ->
+   (_GHC.Base.<_  k2 k = true) /\ 
+  (forall k3, (_GHC.Base.<_  k3 k = true) /\ (k2 == k3 = false) /\
+  sem m k3 <> None -> (_GHC.Base.<_  k3 k2 = true)).
+Proof.
+  intros. pose proof (goJustLT_nothing_between k k1 v1 m lb ub k2 v2 H H0 H1).
+  split. eapply goJustLT_pres_smaller. apply H. apply H0. apply H1. intros.
+  specialize (H2 k3). destruct H3. destruct H4.
+  destruct (_GHC.Base.<_ k3 k2 ) eqn : ?.
+  - reflexivity.
+  - assert (sem m k3 = None). apply H2. split. order e. order e. contradiction.
+Qed.
+
+Lemma goJustLt_val_in_map: forall k k1 v1 m lb ub k2 v2,
+  Bounded m lb ub ->
+  goJustLT k k1 v1 m = Some (k2, v2) ->
+  sem m k2 = Some v2 \/ ((k2 == k1 = true) /\ v2 = v1).
+Proof.
+  intros. generalize dependent k2. revert k k1 v1 v2. induction H; intros.
+  - simpl in H0. inversion H0; subst. right. split. apply Eq_Reflexive. reflexivity.
+  - simpl. simpl in H5. destruct (_GHC.Base.<=_ k x) eqn : ?.
+    + specialize (IHBounded1 k k1 v1 v2 k2 H5). destruct IHBounded1.
+      * rewrite H6. simpl. left. reflexivity.
+      * right. apply H6.
+    + assert (_GHC.Base.<_ x k = true) by (order e).
+      pose proof goJustLT_bounded. specialize (H7 k x v s2 k2 v2 (Some x) ub x k H0 H6 H5).
+      destruct H7. assert (_GHC.Base.<=_ x k2 = true). apply H7. split. reflexivity. order e.
+      assert (sem s1 k2 = None). eapply sem_outside_above. eassumption. solve_Bounds. rewrite H10.
+      simpl. specialize (IHBounded2 k x v v2 k2 H5). destruct IHBounded2.
+      * assert (k2 == x = false) by (solve_Bounds). rewrite H12. simpl. left.
+        assumption.
+      * destruct H11.  left. rewrite H11. simpl. subst. reflexivity.
+Qed. 
+
+Lemma goJustLt_never_none: forall k k1 v1 m,
+  goJustLT k k1 v1 m <> None.
+Proof.
+  intros. revert k k1 v1. induction m; intros.
+  - simpl. destruct (_GHC.Base.<=_ k0 k ). apply IHm1. apply IHm2.
+  - simpl. intro contra. discriminate contra.
+Qed. 
+
+(*Part 1 of the spec: If lookupLT returns a k1, v1 pair, then (k1, v1) is in the map
+  and k1 is the largest key smaller than k*)
+Lemma lookupLT_spec_Some:
+  forall m lb ub k (k1: e) v1, Bounded m lb ub ->
+  lookupLT k m = Some (k1, v1) ->
+  sem m k1 = Some v1 /\ (_GHC.Base.<_  k1 k = true) /\ 
+  (forall k2, (_GHC.Base.<_  k2 k = true) /\ (k1 == k2 = false) /\
+  sem m k2 <> None -> (_GHC.Base.<_  k2 k1 = true)).
+Proof.
+  intros. rewrite <- lookupLT_equiv in H0. generalize dependent k. revert k1 v1. induction H; intros; split; intros.
+  - inversion H0.
+  - inversion H0.
+  - simpl in H5. simpl. destruct (_GHC.Base.<=_  k x) eqn : ?.
+    + apply IHBounded1 in H5. destruct H5. rewrite H5. simpl. reflexivity. 
+    + assert ( _GHC.Base.<_ x k = true) by (order e).
+      pose proof (goJustLT_finds_upper_bound k x v s2 (Some x) ub k1 v1 H0 H6 H5).
+      destruct H7. specialize (H8 x).  
+      pose proof (goJustLt_val_in_map k x v s2 (Some x) ub k1 v1 H0 H5). 
+      pose proof goJustLT_bounded. specialize (H10 k x v s2 k1 v1 (Some x) ub x k H0 H6 H5). 
+      destruct H10. assert (_GHC.Base.<=_ x k1 = true). apply H10. split. reflexivity. order e.
+      assert (sem s1 k1 = None). eapply sem_outside_above. eassumption. solve_Bounds.
+      rewrite H13. simpl. destruct H9.
+      * assert (k1 == x = false) by (solve_Bounds). rewrite H14. simpl. assumption.
+      * destruct H9. subst. rewrite H9. reflexivity.
+  - simpl in H5. destruct (_GHC.Base.<=_ k x) eqn : ?. 
+    + simpl. specialize (IHBounded1 k1 v1 k H5). destruct IHBounded1. destruct H7. split.
+      assumption. intros. apply H8. destruct H9. destruct H10.
+      split. assumption. split. assumption. assert (k2 == x = false) by (order e). 
+      assert (sem s2 k2 = None). eapply sem_outside_below. eassumption. solve_Bounds.
+      rewrite H13 in H11. rewrite H12 in H11. simpl in H11. repeat (rewrite oro_None_r in H11).
+      assumption.
+    + assert (_GHC.Base.<_ x k = true) by (order e). split. eapply goJustLT_pres_smaller. apply H0.
+      apply H6. apply H5. intros. destruct H7. destruct H8. simpl in H9.
+      pose proof goJustLT_bounded. specialize (H10 k x v s2 k1 v1 (Some x) ub x k H0 H6 H5). 
+      destruct H10. assert (_GHC.Base.<=_ x k1 = true). apply H10. split. reflexivity.
+      order e. destruct (compare k2 k1) eqn : ?.
+      order e.
+      order e.
+      assert (k2 == x = false) by (order e). rewrite H13 in H9. simpl in H9.
+      assert (sem s1 k2 = None). eapply sem_outside_above. eassumption. solve_Bounds.
+      rewrite H14 in H9. simpl in H9. eapply goJustLT_finds_upper_bound.
+       apply H0. apply H6. apply H5. split; try(assumption); split; assumption.
+Qed.
+
+(*Part 2: If lookupLT returns None, then every key in the map is smaller than k*)
+Lemma lookupLT_spec_None:
+  forall m lb ub k, Bounded m lb ub ->
+  lookupLT k m = None ->
+  (forall k2 v2, sem m k2 = Some v2 -> _GHC.Base.<=_ k k2 = true).
+Proof.
+  intros. generalize dependent k2. generalize dependent k. revert v2. induction H; intros.
+  - inversion H1.
+  - rewrite <- lookupLT_equiv in H5. simpl in H5. destruct (_GHC.Base.<=_ k x) eqn : ?.
+    simpl in H6. destruct (sem s1 k2) eqn : ?.  
+    * simpl in H6; inversion H6; subst. eapply IHBounded1. apply H5. apply Heqo.
+    * simpl in H6. destruct (k2 == x) eqn : ?.
+      -- order e.
+      -- simpl in H6. solve_Bounds.
+    * assert (goJustLT k x v s2 <> None). apply goJustLt_never_none. rewrite H5 in H7.
+      contradiction.
+Qed.
+
+(** ** Verification of [lookupLE] *)
+Fixpoint goJustLE k (k1: e) v1 (m : Map e a) : option (e * a) :=
+  match m with
+  | Tip => Some (k1, v1)
+  | Bin sz k2 v2 l r => match compare k k2 with
+                        | Lt => goJustLE k k1 v1 l
+                        | Eq => Some (k2, v2)
+                        | Gt => goJustLE k k2 v2 r
+                        end
+  end.
+
+Fixpoint lookupLE' k (m : Map e a) :=
+  match m with
+  | Tip => None
+  | Bin sz k1 v1 l r => match compare k k1 with
+                        | Lt => lookupLE' k l
+                        | Eq => Some (k1, v1)
+                        | Gt => goJustLE k k1 v1 r
+                        end 
+  end.
+
+Lemma lookupLE_equiv:
+  forall m k,
+  lookupLE' k m = lookupLE k m.
+Proof.
+  intros. unfold lookupLE'. unfold lookupLE. unfold goJustLE. reflexivity.
+Qed.
+
+Lemma goJustLE_pres_smaller: forall k k1 v1 m k2 v2 lb ub,
+  Bounded m lb ub ->
+  _GHC.Base.<_ k1 k = true ->
+  goJustLE k k1 v1 m = Some (k2, v2) ->
+  _GHC.Base.<=_ k2 k = true.
+Proof.
+  intros. generalize dependent k1. revert v1 v2 k2 k. induction H; intros.
+  - simpl in H1. inversion H1; subst. order e. 
+  - simpl in H6. destruct (compare k x) eqn : ?.
+    + inversion H6; subst. order e.
+    + eapply IHBounded1. eassumption. eassumption.
+    + assert (_GHC.Base.<_ x k = true) by (order e). eapply IHBounded2. apply H7.
+      apply H6.
+Qed.
+
+Lemma goJustLE_bounded: forall k k1 v1 m k2 v2 lb ub l u,
+  Bounded m lb ub ->
+  _GHC.Base.<_ k1 k = true ->
+  goJustLE k k1 v1 m = Some (k2, v2) ->
+  (lb = Some l /\ _GHC.Base.<=_ l k1 = true -> _GHC.Base.<=_ l k2 = true ) 
+  /\ (ub = Some u /\ _GHC.Base.<=_ k1 u = true -> _GHC.Base.<=_ k2 u = true).
+Proof.
+  intros. generalize dependent k1. revert k v1 k2 v2 u l. induction H; intros.
+  - simpl in H1. inversion H1; subst. split; intros; subst; solve_Bounds.
+  - simpl in H6. destruct (compare k x) eqn : ?.
+    + inversion H6; subst. split; intros. order e. destruct H3. subst. solve_Bounds.
+    + split; intros; subst.  specialize (IHBounded1 _ _ _ _ u l _ H5 H6). destruct IHBounded1.
+       apply H3. apply H7. specialize (IHBounded1 _ _ _ _ x l  _ H5 H6). destruct IHBounded1.
+        destruct H7; subst. assert (Some x = Some x /\ _GHC.Base.<=_ k1 x = true).
+        split. reflexivity. order e. apply H8 in H7.  assert (compare x u = Lt) by (solve_Bounds). 
+        order e.
+    + assert (_GHC.Base.<_ x k = true) by (order e).  split; intros; subst. 
+      specialize (IHBounded2  _ _ _ _ u x _ H7 H6). destruct IHBounded2. 
+      destruct H8; subst. assert (_GHC.Base.<=_ x k2 = true). apply H3. split. reflexivity.
+      order e. assert (_GHC.Base.<_ l x = true) by (solve_Bounds). order e.
+      specialize (IHBounded2 _ _ _ _ u l _ H7 H6). destruct IHBounded2. apply H9.
+      split. apply H8. destruct H8. subst. solve_Bounds.
+Qed. 
+
+Lemma goJustLE_nothing_between: forall k k1 v1 m lb ub k2 v2,
+  Bounded m lb ub ->
+  _GHC.Base.<_ k1 k = true ->
+  goJustLE k k1 v1 m = Some (k2, v2) ->
+  (forall i, compare k2 i = Lt /\ compare i k = Lt ->
+  sem m i = None).
+Proof.
+  intros. generalize dependent i. generalize dependent k2. generalize dependent k1.
+  revert k v1 v2.
+  induction H; intros.
+  - reflexivity.
+  - simpl. simpl in H6. destruct (compare k x) eqn : ?.
+    + assert (i == x = false) by (order e). rewrite H8. assert (sem s2 i = None). {
+      eapply sem_outside_below. eassumption. solve_Bounds. } rewrite H9.
+      simpl. repeat(rewrite oro_None_r). inversion H6; subst. eapply sem_outside_above.
+      eassumption. solve_Bounds. 
+    + assert (i == x = false) by (order e). rewrite H8. assert (sem s2 i = None). {
+      eapply sem_outside_below. eassumption. solve_Bounds. } rewrite H9.
+      simpl. repeat(rewrite oro_None_r).  eapply IHBounded1. apply H5. apply H6.
+      assumption.
+    + assert (_GHC.Base.<_ x k = true) by (order e).
+      pose proof goJustLE_bounded. specialize (H9 _ _ _ _ _ _ _ _ x k H0 H8 H6).
+      destruct H9. assert (_GHC.Base.<=_ x k2 = true). apply H9. split. reflexivity.
+      order e. assert (_GHC.Base.<_ x i = true). order e. assert (sem s1 i = None).
+      eapply sem_outside_above. eassumption. solve_Bounds. rewrite H13.
+      assert (i == x = false) by (order e). rewrite H14. simpl. eapply IHBounded2.
+      apply H8. apply H6. apply H7.
+Qed.
+
+Lemma goJustLE_finds_upper_bound: forall k k1 v1 m lb ub k2 v2,
+  Bounded m lb ub ->
+  _GHC.Base.<_ k1 k = true ->
+  goJustLE k k1 v1 m = Some (k2, v2) ->
+   (_GHC.Base.<=_  k2 k = true) /\ 
+  (forall k3, (_GHC.Base.<_  k3 k = true) /\ (k2 == k3 = false) /\
+  sem m k3 <> None -> (_GHC.Base.<_  k3 k2 = true)).
+Proof.
+  intros. pose proof (goJustLE_nothing_between k k1 v1 m lb ub k2 v2 H H0 H1).
+  split. eapply goJustLE_pres_smaller. apply H. apply H0. apply H1. intros.
+  specialize (H2 k3). destruct H3. destruct H4.
+  destruct (_GHC.Base.<_ k3 k2 ) eqn : ?.
+  - reflexivity.
+  - assert (sem m k3 = None). apply H2. split. order e. order e. contradiction.
+Qed.
+
+Lemma goJustLE_val_in_map: forall k k1 v1 m lb ub k2 v2,
+  Bounded m lb ub ->
+  goJustLE k k1 v1 m = Some (k2, v2) ->
+  sem m k2 = Some v2 \/ ((k2 == k1 = true) /\ v2 = v1).
+Proof.
+  intros. generalize dependent k2. revert k k1 v1 v2. induction H; intros.
+  - simpl in H0. inversion H0; subst. right. split. apply Eq_Reflexive. reflexivity.
+  - simpl. simpl in H5. destruct (compare k x) eqn : ?.
+    + inversion H5; subst. assert (sem s1 k2 = None). eapply sem_outside_above.
+      eassumption. solve_Bounds. rewrite H3. rewrite Eq_Reflexive. simpl.
+      left. reflexivity. 
+    + specialize (IHBounded1 k k1 v1 v2 k2 H5). destruct IHBounded1.
+      * rewrite H6. simpl. left. reflexivity.
+      * right. apply H6.
+    + assert (_GHC.Base.<_ x k = true) by (order e).
+      pose proof goJustLE_bounded. specialize (H7 k x v s2 k2 v2 (Some x) ub x k H0 H6 H5).
+      destruct H7. assert (_GHC.Base.<=_ x k2 = true). apply H7. split. reflexivity. order e.
+      assert (sem s1 k2 = None). eapply sem_outside_above. eassumption. solve_Bounds. rewrite H10.
+      simpl. specialize (IHBounded2 k x v v2 k2 H5). destruct IHBounded2.
+      * assert (k2 == x = false) by (solve_Bounds). rewrite H12. simpl. left.
+        assumption.
+      * destruct H11.  left. rewrite H11. simpl. subst. reflexivity.
+Qed. 
+
+Lemma goJustLE_never_none: forall k k1 v1 m,
+  goJustLE k k1 v1 m <> None.
+Proof.
+  intros. revert k k1 v1. induction m; intros.
+  - simpl. destruct (compare k0 k) eqn : ?.
+    + intro contra. discriminate contra.
+    + apply IHm1.
+    + apply IHm2.
+  - simpl. intro contra. discriminate contra.
+Qed. 
+
+(*Part 1 of the spec: If lookupLT returns a k1, v1 pair, then (k1, v1) is in the map
+  and k1 is the largest key less than or equal to than k*)
+Lemma lookupLE_spec_Some:
+  forall m lb ub k (k1: e) v1, Bounded m lb ub ->
+  lookupLE k m = Some (k1, v1) ->
+  sem m k1 = Some v1 /\ (_GHC.Base.<=_  k1 k = true) /\ 
+  (forall k2, (_GHC.Base.<_  k2 k = true) /\ (k1 == k2 = false) /\
+  sem m k2 <> None -> (_GHC.Base.<_  k2 k1 = true)).
+Proof.
+  intros. rewrite <- lookupLE_equiv in H0. generalize dependent k. revert k1 v1. induction H; intros; split; intros.
+  - inversion H0.
+  - inversion H0.
+  - simpl in H5. simpl. destruct (compare k x) eqn : ?.
+    + inversion H5; subst. assert (sem s1 k1 = None). eapply sem_outside_above. eassumption.
+      solve_Bounds. rewrite H3. rewrite Eq_Reflexive. reflexivity.
+    + apply IHBounded1 in H5. destruct H5. rewrite H5. simpl. reflexivity. 
+    + assert ( _GHC.Base.<_ x k = true) by (order e).
+      pose proof (goJustLE_finds_upper_bound k x v s2 (Some x) ub k1 v1 H0 H6 H5).
+      destruct H7. specialize (H8 x).  
+      pose proof (goJustLE_val_in_map k x v s2 (Some x) ub k1 v1 H0 H5). 
+      pose proof goJustLE_bounded. specialize (H10 k x v s2 k1 v1 (Some x) ub x k H0 H6 H5). 
+      destruct H10. assert (_GHC.Base.<=_ x k1 = true). apply H10. split. reflexivity. order e.
+      assert (sem s1 k1 = None). eapply sem_outside_above. eassumption. solve_Bounds.
+      rewrite H13. simpl. destruct H9.
+      * assert (k1 == x = false) by (solve_Bounds). rewrite H14. simpl. assumption.
+      * destruct H9. subst. rewrite H9. reflexivity.
+  - simpl in H5. destruct (compare k x ) eqn : ?.
+    + inversion H5; subst. split. order e. intros. order e. 
+    + simpl. specialize (IHBounded1 k1 v1 k H5). destruct IHBounded1. destruct H7. split.
+      assumption. intros. apply H8. destruct H9. destruct H10.
+      split. assumption. split. assumption. assert (k2 == x = false) by (order e). 
+      assert (sem s2 k2 = None). eapply sem_outside_below. eassumption. solve_Bounds.
+      rewrite H13 in H11. rewrite H12 in H11. simpl in H11. repeat (rewrite oro_None_r in H11).
+      assumption.
+    + assert (_GHC.Base.<_ x k = true) by (order e). split. eapply goJustLE_pres_smaller. apply H0.
+      apply H6. apply H5. intros. destruct H7. destruct H8. simpl in H9.
+      pose proof goJustLE_bounded. specialize (H10 k x v s2 k1 v1 (Some x) ub x k H0 H6 H5). 
+      destruct H10. assert (_GHC.Base.<=_ x k1 = true). apply H10. split. reflexivity.
+      order e. destruct (compare k2 k1) eqn : ?.
+      order e.
+      order e.
+      assert (k2 == x = false) by (order e). rewrite H13 in H9. simpl in H9.
+      assert (sem s1 k2 = None). eapply sem_outside_above. eassumption. solve_Bounds.
+      rewrite H14 in H9. simpl in H9. eapply goJustLE_finds_upper_bound.
+       apply H0. apply H6. apply H5. split; try(assumption); split; assumption.
+Qed.
+
+Lemma goJustLE_spec_eq: forall m lb ub k v k' v',
+  Bounded m lb ub ->
+  sem m k = Some v ->
+  (exists k1, k1 == k = true /\ goJustLE k k' v' m = Some (k1, v)).
+Proof.
+  intros. generalize dependent k. revert v k' v'. induction H; intros.
+  - inversion H0.
+  - simpl in H5. simpl. destruct (sem s1 k) eqn : ?. 
+    + assert (compare k x = Lt) by (solve_Bounds).
+      rewrite H6. apply IHBounded1. simpl in H5. inversion H5; subst. assumption.
+    + simpl in H5. destruct (k == x) eqn : ?. assert (compare k x = Eq) by (order e).
+      * rewrite H6. exists x. split. order e. inversion H5. reflexivity.
+      * simpl in H5. assert (compare k x = Gt) by (solve_Bounds). rewrite H6.
+        apply IHBounded2. assumption.
+Qed.
+
+(*Part 2: If the value is in the map, lookupLE returns it*)
+Lemma lookupLE_spec_eq: forall m lb ub k v,
+  Bounded m lb ub ->
+  sem m k = Some v ->
+  (exists k1, k1 == k = true /\ lookupLE k m = Some (k1, v)).
+Proof.
+  intros. generalize dependent k. revert v. induction H; intros.
+  - inversion H0.
+  - simpl in H5. rewrite <- lookupLE_equiv. simpl.
+    destruct (sem s1 k) eqn : ?.
+    + assert (compare k x = Lt) by (solve_Bounds). rewrite H6. apply IHBounded1.
+      simpl in H5. inversion H5; subst. assumption.
+    + simpl in H5. destruct (k == x) eqn : ?.
+      * simpl in H5. exists x. split. order e. assert (compare k x = Eq) by (order e).
+        rewrite H6. inversion H5; subst. reflexivity.
+      * simpl in H5. assert (compare k x = Gt) by (solve_Bounds). rewrite H6.
+        eapply goJustLE_spec_eq. eassumption. assumption.
+Qed.
+    
+(*Part 3: If lookupLT returns None, then every key in the map is smaller than k*)
+Lemma lookupLE_spec_None:
+  forall m lb ub k, Bounded m lb ub ->
+  lookupLE k m = None ->
+  (forall k2 v2, sem m k2 = Some v2 -> _GHC.Base.<_ k k2 = true).
+Proof.
+  intros. generalize dependent k2. generalize dependent k. revert v2. induction H; intros.
+  - inversion H1.
+  - rewrite <- lookupLE_equiv in H5. simpl in H5. destruct (compare k x) eqn : ?.
+    + simpl in H6. order e. 
+    + simpl in H6. destruct (sem s1 k2) eqn : ?.  
+      * simpl in H6; inversion H6; subst. eapply IHBounded1. apply H5. apply Heqo.
+      * simpl in H6. destruct (k2 == x) eqn : ?.
+      -- order e.
+      -- simpl in H6. solve_Bounds.
+    + assert (goJustLE k x v s2 <> None). apply goJustLE_never_none. rewrite H5 in H7.
+      contradiction.
+Qed.
+
+(*TODO: see about lookupGE and lookupGT: the proofs will be the same but with > instead of <*)
 
 (** ** Verification of [insert] *)
 
@@ -1356,6 +1810,140 @@ Proof.
         applyDesc balanceR_Desc;
         solve_Desc.
 Qed.
+
+(** ** Verification of [insertWith] *)
+Lemma insertWith_Desc:
+  forall (f: a -> a -> a) y v s lb ub,
+  Bounded s lb ub ->
+  isLB lb y = true ->
+  isUB ub y = true ->
+  Desc (insertWith f y v s) lb ub (if isSome (sem s y) then size s else (1 + size s)%Z)
+      (fun i => (if i == y then match (sem s y) with
+                                | None => Some v
+                                | Some x => Some (f v x)
+                                end  else None ||| sem s i )).
+Proof.
+  intros ?????? HB HLB HUB.
+  induction HB; intros.
+  * simpl.
+    applyDesc singleton_Desc; try eassumption; solve_Desc.
+  * subst; cbn -[Z.add].
+    destruct (compare y x) eqn:?.
+    + rewrite compare_Eq in *.
+      rewrite Heqc.
+      rewrite ?isSome_oro, ?isSome_Some, ?orb_true_r, ?orb_true_l.
+      solve_Desc.
+    + clear IHHB2.
+      applyDesc IHHB1.
+      rewrite (sem_outside_below HB2) by order_Bounds.
+      replace (y == x) with false by order_Bounds.
+      simpl_options. destruct (sem s1 y) eqn:?; simpl isSome in *; try lia;
+      applyDesc balanceL_Desc; solve_Desc.
+    + clear IHHB1.
+      applyDesc IHHB2.
+      rewrite (sem_outside_above HB1) by order_Bounds.
+      replace (y == x) with false by order_Bounds.
+      simpl_options. destruct (sem s2 y) eqn:?; simpl_options; try lia; applyDesc balanceR_Desc;
+      solve_Desc.
+Qed.
+
+(** ** Verification of [insertWithKey] *)
+Lemma insertWithKey_Desc:
+  forall (f: e -> a -> a -> a) y v s lb ub,
+  Bounded s lb ub ->
+  isLB lb y = true ->
+  isUB ub y = true ->
+  Desc (insertWithKey f y v s) lb ub (if isSome (sem s y) then size s else (1 + size s)%Z)
+      (fun i => (if i == y then match (sem s y) with
+                                | None => Some v
+                                | Some x => Some (f y v x)
+                                end  else None ||| sem s i )).
+Proof.
+  intros ?????? HB HLB HUB.
+  induction HB; intros.
+  * simpl.
+    applyDesc singleton_Desc; try eassumption; solve_Desc.
+  * subst; cbn -[Z.add].
+    destruct (compare y x) eqn:?.
+    + rewrite compare_Eq in *.
+      rewrite Heqc.
+      rewrite ?isSome_oro, ?isSome_Some, ?orb_true_r, ?orb_true_l.
+      solve_Desc.
+    + clear IHHB2.
+      applyDesc IHHB1.
+      rewrite (sem_outside_below HB2) by order_Bounds.
+      replace (y == x) with false by order_Bounds.
+      simpl_options. destruct (sem s1 y) eqn:?; simpl isSome in *; try lia;
+      applyDesc balanceL_Desc; solve_Desc.
+    + clear IHHB1.
+      applyDesc IHHB2.
+      rewrite (sem_outside_above HB1) by order_Bounds.
+      replace (y == x) with false by order_Bounds.
+      simpl_options. destruct (sem s2 y) eqn:?; simpl_options; try lia; applyDesc balanceR_Desc;
+      solve_Desc.
+Qed.
+
+(** ** Verification of [insertLookupWithKey] *)
+Lemma pair_fst_snd: forall {a: Type} {b : Type} (p : a * b),
+   p = (fst p, snd p).
+Proof.
+  intros. destruct p. simpl. reflexivity.
+Qed.
+
+Lemma insertLookupWithKey_lookup:
+  forall m lb ub f k v1,
+  Bounded m lb ub ->
+  sem m k = fst ((insertLookupWithKey f k v1 m)).
+Proof.
+  intros. generalize dependent k. revert f v1. induction H; intros.
+  - simpl. reflexivity.
+  - simpl.   destruct (sem s1 k) eqn : ?.
+   + assert (compare k x = Lt) by (solve_Bounds). rewrite H5. simpl. 
+     rewrite (pair_fst_snd (insertLookupWithKey f k v1 s1 )). simpl.
+     rewrite <- Heqo. apply IHBounded1.
+   + simpl. destruct (k == x) eqn : ?.
+      * simpl. assert (compare k x = Eq) by (order e).
+        rewrite H5. simpl. reflexivity.
+      * simpl. destruct (sem s2 k) eqn : ?.
+        -- assert (compare k x = Gt) by (solve_Bounds). rewrite H5. 
+           rewrite (pair_fst_snd (insertLookupWithKey f k v1 s2 )). simpl.
+           rewrite <- Heqo0. apply IHBounded2.
+        -- destruct (compare k x) eqn : ?.
+          ++ order e.
+          ++ rewrite (pair_fst_snd (insertLookupWithKey f k v1 s1)). simpl.
+             rewrite <- Heqo. apply IHBounded1.
+          ++ rewrite (pair_fst_snd (insertLookupWithKey f k v1 s2)). simpl.
+             rewrite <- Heqo0. apply IHBounded2.
+Qed.
+
+(*This makes the Desc incredibly easy*)
+Lemma insertWithKey_insertLookupWithKey: forall (m: Map e a) f k v,
+  insertWithKey f k v m = snd(insertLookupWithKey f k v m).
+Proof.
+  intros m. induction m; intros.
+  - simpl. destruct (compare k0 k).
+    + simpl. reflexivity.
+    + simpl. rewrite (pair_fst_snd (insertLookupWithKey f k0 v m1)). simpl.
+      rewrite IHm1. reflexivity.
+    + rewrite (pair_fst_snd (insertLookupWithKey f k0 v m2)). simpl.
+      rewrite IHm2. reflexivity.
+  - simpl. reflexivity.
+Qed.  
+
+Lemma insertLookupWithKey_Desc:
+  forall (f: e -> a -> a -> a) y v s lb ub,
+  Bounded s lb ub ->
+  isLB lb y = true ->
+  isUB ub y = true ->
+  Desc (snd(insertLookupWithKey f y v s)) lb ub (if isSome (sem s y) then size s else (1 + size s)%Z)
+      (fun i => (if i == y then match (sem s y) with
+                                | None => Some v
+                                | Some x => Some (f y v x)
+                                end  else None ||| sem s i )).
+Proof.
+  intros. rewrite <- insertWithKey_insertLookupWithKey. apply insertWithKey_Desc; assumption.
+Qed. 
+
 
 (** ** Verification of [insertR] *)
 
@@ -8146,7 +8734,7 @@ Proof.
     + assert (exists v, sem m x0 = Some v). exists e. assumption.
       pose proof (map2_map_part_1_in _ _ _ _ _ _ f H H0 H3). rewrite H4.
       rewrite Heqo. reflexivity.
-    + assert (sem (map2_map_part1 elt elt' elt'' m m' f) x0 = None).
+    + assert (sem (map2_map_part1 elt0 elt' elt'' m m' f) x0 = None).
       unfold map2_map_part1. rewrite <- map_none_spec. apply Heqo. apply H.
       rewrite H3. reflexivity.
   - unfold map2_map_part1. apply mapWithKey_pres_WF. apply H.
@@ -8163,9 +8751,9 @@ Lemma map2_map_notin: forall (elt elt' elt'' : Type)(m: Map key elt) (m': Map ke
 Proof.
   intros. rewrite map2_map_equiv. unfold map2_map_alt. erewrite sem_union_equiv.
   unfold sem_union. destruct H1. 
-  assert (sem (map2_map_part1 elt elt' elt'' m m' f) x0 = None). { 
+  assert (sem (map2_map_part1 elt0 elt' elt'' m m' f) x0 = None). { 
   apply map2_map_part_1_notin; assumption. }
-  assert (sem (map2_map_part2 elt elt' elt'' m m' f) x0 = None). { 
+  assert (sem (map2_map_part2 elt0 elt' elt'' m m' f) x0 = None). { 
   apply map2_map_part_2_notin; assumption. }
   rewrite H3. rewrite H4. reflexivity. 
   unfold map2_map_part1. apply mapWithKey_pres_WF. apply H.
